We know,
\begin{align}
    \pr{A|B} = \frac{\pr{A\cap B}}{\pr{B}}
\end{align}
Also, for a Poisson Distribution:
\begin{align}
    \pr{N = x} = \frac{e^{-\lambda}\lambda^x}{x!}
    \label{poisson}
\end{align}
where $\lambda$ is the parameter\\
Let $N_2$ be the number of persons hospitalised.\\
Let $N = a$, and $N_1 = i(i\leq a)$, then, $N_2 = a-i$\\
Then, from \eqref{condition} and \eqref{poisson}:
\begin{align}
    \pr{N_2 = a-i} =\pr{N_1 = i}\\
    =\pr{N_1 = i|N = a}\pr{N = a}\\
     = \frac{1}{a}\frac{e^{-\lambda}\lambda^a}{a!}
\end{align}
Thus,
\begin{align}
    E(N_2) = \sum_{a = 0}^{\infty} \sum_{i = 0 }^{a} (a-i) \times \frac{1}{a}\frac{e^{-\lambda}\lambda^a}{a!}\\
     = \sum_{a=0}^{\infty}\frac{e^{-\lambda}\lambda^a}{a!} \sum_{i = 0 }^{a} \frac{a-i}{a}\\
    = \sum_{a=0}^{\infty}\frac{e^{-\lambda}\lambda^a}{a!} \brak{a - \frac{(a+1)}{2}}\\
     = \sum_{a=0}^{\infty}\frac{e^{-\lambda}\lambda^a}{a!}\frac{a-1}{2}\\
      = \frac{e^{-\lambda}}{2}\sbrak{\sum_{a=0}^{\infty}\frac{a\lambda^a}{a!} - \sum_{a=0}^{\infty}\frac{\lambda^a}{a!}}\\
       = \frac{e^{-\lambda}}{2}\sbrak{\lambda\sum_{a=1}^{\infty} \frac{\lambda^{a-1}}{(a-1)!} - \sum_{a=0}^{\infty}\frac{\lambda^a}{a!}}\\
        = \frac{e^{-\lambda}}{2}\sbrak{\lambda e^\lambda - e^\lambda}\\
         = \frac{\lambda - 1}{2}
\end{align}