
Let X be the random variable. To find 
\begin{align}
    \frac{4}{3} E[X(X^2 -15X + 27)]
\end{align}
Let,
\begin{align}
    g(X) &= X(X^2 -15X + 27)  \\
         &= X^3 -15X^2 + 27X
\end{align}
Then for random variable X we have that,
\begin{align}
    E[g(X)] = \int_{-\infty}^{\infty} g(x)f(x) \,dx
\end{align}
The probability distribution of X is,
\begin{align}
\label{st2021-22:eq:spdf_X}
f\brak{x} = 
\begin{cases}
\frac{3}{13}(1-x)(9-x) & 0 < x < 1
\\
0 & \text{ otherwise}
\end{cases}
\end{align}
Using \ref{st2021-22:eq:spdf_X} we have,
\begin{align}
    E[g(X)] &= 0 +\int_{0}^{1} g(x)f(x) \,dx + 0
\end{align}
Where ,
\begin{align}
    f(x ) &= \frac{3}{13}(1-x)(9-x) \text{ and}  \\
    g(x) &= x^3 -15x^2 + 27x
\end{align}
Using Integration by substitution let,
\begin{align*}
    t &= x^3 - 15x^2 + 27x \\
    \,dt &= 3x^2 - 30x + 27 \\
         &= 3(1-x)(9-x)
\end{align*}
The corresponding limits are,
\begin{align}
    \text{For } x &=0  \implies t = 0^3 -15\times 0^2 + 27 \times 0 = 0 \\
        \text{For } x &=1  \implies t = 1^3 -15\times 1^2 + 27 \times 1 = 13
\end{align}
Therefore we have,
\begin{align}
    E[g(X)] &= \frac{1}{13} \int_{0}^{13} t \,dt \\
    & = \frac{1}{13} \times \brak{\frac{t^2}{2}}  \Biggr|_{0}^{13} \\
    &= \frac{1}{13} \times \frac{13^2}{2} \\
    & = \frac{13}{2} 
\end{align}
Thus, 
\begin{align}
    \frac{4}{3} E[g(X)] & =  \frac{4}{3} \times \frac{13}{2} \\
    &= \frac{26}{3} \\
    &= 8.67  \text{ (rounded off)}
\end{align}
Therefore,
\begin{align}
    \frac{4}{3} E[X(X^2 -15X + 27)] & =  8.67
\end{align}