
Probability mass function of a trinomial  distribution is :
\begin{multline}
   \p{x}{y} \\=\brak{\frac{7!}{x!y!(7-x-y)!}}(0.6)^x(0.2)^y(0.2)^{7-x-y}\\
  \nonumber  =\brak{\frac{7!}{x!(7-x)!}\frac{(7-x)!}{y!(7-x-y)!}}(0.6)^x(0.2)^y(0.2)^{7-x-y}
\end{multline}
\begin{equation}
    \p{x}{y}=\comb{7}{x}\comb{7-x}{y}(0.6)^x(0.2)^y(0.2)^{7-x-y}\label{1}
\end{equation}
Using \eqref{1}, $\q{x}$ is 
\begin{align}
   \nonumber \q{x}&=\sum_{y=0}^{7-x} \p{x}{y}\\
  \nonumber &=\comb{7}{x}(0.6)^x\,\sum_{y=0}^{7-x}\, \comb{7-x}{y} (0.2)^y(0.2)^{7-x-y} \\
  \nonumber  &=\comb{7}{x}(0.6)^x\,{(0.4)^{7-x}}\\
    \q{x}&=\comb{7}{x}(0.6)^x\,{(0.4)^{7-x}}\label{2}
\end{align}
We have to find $\mean{Y|X=3}$ ,
\begin{align}
    \mean{Y|X=3}&=\sum_{y=0}^4 \: y P(Y=y|X=3)\\
    \mean{Y|X=3}&=\sum_{y=0}^4 y \brak{  \frac{ \p{3}{y}}{P(X=3)} }\label{3}
\end{align}
By taking X=3 in \eqref{1} and \eqref{2}  to use in \eqref{3},
\begin{align}
   \nonumber \mean{Y|X=3}&=\sum_{y=0}^4 y \brak{ \frac{ \p{3}{y}}{P(X=3)}}\\
  \nonumber  &=\sum_{y=0}^4 y   \brak{\frac{\comb{7}{3}\comb{4}{y}(0.6)^3(0.2)^y(0.2)^{4-y}}{\comb{7}{3}(0.6)^3\,{(0.4)^{4}}}}\\
 \nonumber &=\sum_{y=0}^4 y   \brak{\frac{\comb{4}{y}(0.2)^{4}}{{(0.4)^{4}}}}\\
 \mean{Y|X=3}&=\sum_{y=0}^4 {\frac{y(\comb{4}{y})}{{16}}}\label{4}
 \end{align}
 We know that,
 \begin{align}
     \comb{n}{r} = \frac{n}{r}\brak{\comb{n-1}{r-1}}\label{5}
 \end{align}
 Using \eqref{5} in \eqref{4},
 \begin{align}
  \mean{Y|X=3}&=\frac{1}{16}\sum_{y=0}^4\, {y(\comb{4}{y})}\\
  &=\frac{1}{16}\sum_{y=1}^{4} y\brak{\frac{4}{y}}(\comb{3}{y-1})\\
  &=\frac{1}{4}\sum_{k=0}^{3}(\comb{3}{k})\\
  &=\frac{1}{4}(1+1)^3=\frac{1}{4}(8)\\
  \mean{Y|X=3}&=2
\end{align}
Therefore the value of $\mean{Y|X=3}=2$.