
Consider a unit step function $u(x)$,
\begin{align}
u(x) = 
    \begin{cases}
        1 & x \geq 0 \\
        0 & \text{otherwise}
    \end{cases}
\end{align}
We will remove the discontinuity at $x=0$ by defining $u_{\alpha}(x)$ for any $\alpha > 0$,
\begin{align}
u_{\alpha}(x) &= 
    \begin{cases}
        1 & x > \frac{\alpha}{2} \\
        \frac{1}{\alpha}(x + \frac{\alpha}{2}) & -\frac{\alpha}{2} \leq x \leq \frac{\alpha}{2} \\
        0 & x < -\frac{\alpha}{2}
    \end{cases}\\
\delta_{\alpha}(x) &= \frac{du_{\alpha}(x)}{dx}\\
\delta_{\alpha}(x) &=
    \begin{cases}
        \frac{1}{\alpha} & -\frac{\alpha}{2} \leq x \leq \frac{\alpha}{2} \\
        0 & |x| > \frac{\alpha}{2}
    \end{cases}\\
u(x) &= \lim_{\alpha \to 0} u_{\alpha}(x)\\
\delta (x) &= \lim_{\alpha \to 0} \delta_{\alpha}(x)
\end{align}
\begin{align}
    \int_{-\infty}^{\infty}g(x)\delta(x-x_0)dx = g(x_0) \label{ma2015-17:eq:1}
\end{align}
We will add dirac $\delta$ functions to remove discontinuities in $F(x)$.
%We will add $\frac{1}{4}u(x) + \frac{1}{12}u(x - 1) + \frac{1}{6}u(x-2) + \frac{1}{2}u\brak{x-\frac{11}{3}}$ to $F(x)$
\begin{align}
    f_{X}(x) &= \frac{dF(x)}{dx}
\end{align}
\begin{multline}
    f_{X}(x) = \frac{1}{4}\delta(x) + \frac{1}{12}\delta(x - 1) + \frac{1}{6}\delta(x-2) +\\ \frac{1}{2}\delta\brak{x-\frac{11}{3}} + 0
\end{multline}
We will use \eqref{ma2015-17:eq:1} to compute E(X)
\begin{align}
    E(X) = \int_{-\infty}^{\infty}xf_X(x)dx
\end{align}
\begin{multline}
    E(X) = \int_{-\infty}^{\infty}\frac{1}{4}x\delta(x) + \frac{1}{12}x\delta(x - 1) +\\ \frac{1}{6}x\delta(x-2) + \frac{1}{2}x\delta\brak{x-\frac{11}{3}}dx
\end{multline}
\begin{align}
    E(X) &= {\frac{1}{4}}\times 0 + {\frac{1}{12}}\times 1 + {\frac{1}{6}}\times 2 + {\frac{1}{2}}\times{\frac{11}{3}}\\
    E(X) &= 2.25
\end{align}
%
{Alternative Solution: }
\begin{align}
    E(g(X)) = \int_{-\infty}^{\infty} g(x)dF(x)
\end{align}
Suppose $F(x)$ is continuously differentiable on \sbrak{a,b} except at a finite number of points $c_1, c_2, \dots c_n$.\\
\begin{multline}
    \int_{a}^{b}g(x)dF(x) = \int_{a}^{c_1}g(x)dF(x) +\\ g(c_1)\sbrak{F(c_1) - \lim_{\substack{x \to c_1 \\ x < c_1}}F(x)} + \\ \int_{c_1}^{c_2}g(x)dF(x) + \\g(c_2)\sbrak{F(c_2) - \lim_{\substack{x \to c_2 \\ x < c_2}}F(x)} + \dots +\\ \int_{c_{n-1}}^{c_n}g(x)dF(x) +\\ g(c_n)\sbrak{F(c_n) - \lim_{\substack{x \to c_n \\ x < c_n}}F(x)} + \\ \int_{c_n}^{b}g(x)dF(x)
\end{multline}
As per the question, $g(X) = X$
\begin{align}
    E(X) = \int_{-\infty}^{\infty} xdF(x)
\end{align}
\begin{multline}
    E(X) = \int_{-\infty}^{0}xdF(x) + 0\sbrak{F(0) - \lim_{\substack{x \to 0 \\ x < 0}}F(x)} + \\ \int_{0}^{1}xdF(x) + 1\sbrak{F(1) - \lim_{\substack{x \to 1 \\ x < 1}}F(x)} + \\ \int_{1}^{2}xdF(x) + 2\sbrak{F(2) - \lim_{\substack{x \to 2 \\ x < 2}}F(x)} + \\ \int_{2}^{\frac{11}{3}}xdF(x) +  \frac{11}{3}\sbrak{F\brak{\frac{11}{3}} - \lim_{\substack{x \to \frac{11}{3} \\ x < \frac{11}{3}}}F(x)} +\\ \int_{\frac{11}{3}}^{\infty}xdF(x)
\end{multline}
\begin{multline}
    \int_{-\infty}^{0}xdF(x) = \int_{0}^{1}xdF(x) = \int_{1}^{2}xdF(x) = \\ \int_{2}^{\frac{11}{3}}xdF(x) = \int_{\frac{11}{3}}^{\infty}xdF(x) = 0
\end{multline}
\begin{align}
    E(X) = 2.25
\end{align}