Given, $X\sim \mathcal P(\lambda)$ and $Y \sim \mathcal P(\mu)$.
The probability mass functions (PMFs) of random variables X and Y are given by:
\begin{align}
  p_X(x) = 
  \begin{cases}
      \dfrac{e^{-\lambda}\lambda^{x}}{x!}, & \text{for } x=0,1,2,\dots\\
    0, & \text{otherwise } 
  \end{cases}
\end{align}
\begin{align}
  p_Y(y) = 
  \begin{cases}
     \dfrac{e^{-\mu}\mu^{y}}{y!}, & \text{for } y=0,1,2,\dots\\
    0, & \text{otherwise } 
  \end{cases}
\end{align}
where: the parameters $\lambda = 1$ and $\mu = 2$.
As X and Y are independent, we have for $k \geq 0$, the distribution function $p_{X+Y}(k)$ is a convolution of distribution functions $p_X(k)$ and $p_Y(k)$: 
\begin{align}
p_{X+Y}(k) &= \pr{X+ Y = k} = \pr{Y = k - X}\\
&= \sum_{i}\pr{Y = k - i| X=i}\times p_X(i)
\end{align}
After unconditioning, as X and Y are independent: 
\begin{align}
\pr{Y = k - i| X=i} = \pr{Y = k - i} = p_Y(k-i)
\end{align}
\begin{align}
p_{X+Y}(k) &= p_Y(k)*p_X(k)\\ 
    &= \sum_{i=0}^k p_Y(k-i) \times p_X(i)\\
    &= \sum_{i=0}^k e^{-\mu}\frac{\mu^{k-i}}{(k-i)!}e^{-\lambda}\frac{\lambda^i}{i!}\\
   &= e^{-(\mu + \lambda)}\frac 1{k!}\sum_{i=0}^k \frac{k!}{i!(k-i)!}\mu^{k-i}\lambda^i\\
   &= e^{-(\mu + \lambda)}\frac 1{k!}\sum_{i=0}^k \comb{k}{i} \mu^{k-i}\lambda^i\\
   &= \frac{(\mu + \lambda)^k}{k!} \times e^{-(\mu + \lambda)}
\end{align}
Hence,  $X+ Y \sim \mathcal P(\mu + \lambda)$.
\begin{align}
\pr{X=1|X+Y=4} &= \frac{\pr{X=1, Y=3}}{\pr{X+Y=4}}\\
&= \frac{\pr{X=1} \times \pr{Y=3}}{\pr{X+Y=4}} \\
&= \frac{\dfrac{e^{-1}\times1^{1}}{1!} \times \dfrac{e^{-2}\times2^{3}}{3!}}{\dfrac{e^{-3}\times3^{4}}{4!}}\\
&= 4 \times \frac{(1)(2)^{3}}{(3)^{4}}\\
&= \frac{32}{81}\\
&= 0.39506172839
\end{align}