
Given,
\begin{align} \label{ma2001-24:eq-1}
    E(X)=E(Y)=3
\end{align}
\begin{align}
    Var(X)=Var(Y)=1
\end{align}
\begin{align}
    Cov(X,Y)=1/2
\end{align}
Now,
\begin{align}
    Var(X)=E(X^2)-(E(X))^2
\end{align}
Substituting given values, we get,
\begin{align}
    1=E(X^2)-3^2
\end{align}
So,
\begin{align} \label{ma2001-24:eq-2}
    E(X^2)=10
\end{align}
Similarly for $Y$,
\begin{align} \label{ma2001-24:eq-3}
    E(Y^2)=10
\end{align}
Also,
\begin{align}
    Cov(X,Y)=E(XY)-E(X)E(Y)
\end{align}
Substituting given values, we get,
\begin{align}
    1/2=E(XY)-(3)(3)
\end{align}
So,
\begin{align} \label{ma2001-24:eq-4}
    E(XY)=19/2
\end{align}
Let $Z$ be a random variable defined as
\begin{align} \label{ma2001-24:eq-5}
    Z=X-Y
\end{align}
Then using \eqref{ma2001-24:eq-1},
\begin{align} \label{ma2001-24:eq-6}
    E(Z)=E(X-Y)=E(X)-E(Y)=0
\end{align}
Now, using \eqref{ma2001-24:eq-6}
\begin{align}
    Var(Z)=E(Z^2)-(E(Z))^2=E(Z^2)
\end{align}
\begin{align}
    Var(Z)=E((X-Y)^2)
\end{align}
\begin{align}
    Var(Z)=E(X^2)+E(Y^2)-2E(XY)
\end{align}
Using \eqref{ma2001-24:eq-2}, \eqref{ma2001-24:eq-3} and \eqref{ma2001-24:eq-4},
\begin{align}
    Var(Z)=10+10-2 \times 19/2
\end{align}
\begin{align} \label{ma2001-24:eq-7}
    Var(Z)=1
\end{align}
\begin{theorem}
(Chebychev's Inequality)\ Let T be an arbitrary random variable, with finite mean E(T), then for all $a>0$,
\begin{align}
    \pr{|T-E(T)| \geq a} \leq \dfrac{Var(T)}{a^2}
\end{align}
\end{theorem}
\begin{proof}
Let $A$ be a non-negative random variable and $a>0$ be any real number. Define a new random variable $B$ by
\begin{align}
B=  \begin{cases} 
          a & A \geq a \\
          0 & A < a
    \end{cases}
\end{align}
Then clearly $B \leq A$ and by monotonicity,
\begin{align} \label{ma2001-24:eq-8}
    E(B) \leq E(A)
\end{align}
\begin{align}
    E(B)=a\pr{B=a}+0\pr{B=0}
\end{align}
\begin{align} \label{ma2001-24:eq-9}
    E(B)=a\pr{A \geq a}
\end{align}
By \eqref{ma2001-24:eq-8} and \eqref{ma2001-24:eq-9},
\begin{align}
    a\pr{A \geq a} \leq  E(A)
\end{align}
\begin{align} \label{ma2001-24:eq-10}
    \pr{A \geq a} \leq \dfrac{E(A)}{a}
\end{align}
Set $A=(T-E(T))^2$. Then,
\begin{align}
    \pr{|T-E(T)| \geq a}=\pr{A \geq a^2}
\end{align}
Using \eqref{ma2001-24:eq-10},
\begin{align}
    \pr{|T-E(T)| \geq a} \leq \dfrac{E(A)}{a^2}
\end{align}
\begin{align}
    \pr{|T-E(T)| \geq a} \leq \dfrac{E(T-E(T))^2}{a^2}
\end{align}
\begin{align}
    \pr{|T-E(T)| \geq a} \leq \dfrac{Var(T)}{a^2}
\end{align}
\end{proof}
Applying Chebychev's Inequality for $Z$ with $a=6$, we get,
\begin{align}
    \pr{|Z-E(Z)| \geq 6} \leq \dfrac{Var(Z)}{6^2}
\end{align}
Using \eqref{ma2001-24:eq-6} and \eqref{ma2001-24:eq-7},
\begin{align}
    \pr{|Z-0| \geq 6} \leq \dfrac{1}{36}
\end{align}
As $Z=X-Y$,
\begin{align}
    \pr{|X-Y| \geq 6} \leq \dfrac{1}{36}
\end{align}