
According to the question, we want the following events to occur in order: 
\begin{enumerate}
    \item First visitor, $P_1$ arrives while no one leaves
    \item Second visitor $P_2$ arrives while no one leaves
    \item One or more person leaves before the third visitor $P_3$ arrives
\end{enumerate}
Let the above events be $E_1$, $E_2$ and $E_3$ respectively. Thus the required probability
\begin{align}
    &= \pr{E_1E_2E_3}\\
    &= \pr{E_1}\pr{E_2|E_1}\pr{E_3|E_1E_2}\label{st2021-50:Requiredprobability}
\end{align}
\begin{table}
    \centering
    \begin{tabular}{|c|c|}
    \hline
    Symbol  & Representation  \\
    \hline
    $X_1$            & Arrival time of $P_1$  \\
    $X_1+X_2$        & Arrival time of $P_2$  \\
    $X_1+X_2+X_3$    & Arrival time of $P_3$  \\
    \hline
    $Y_1,...,Y_{10}$ & Departure times of the  \\
                     & 10 people in park currently\\
    \hline
    $X_1+Y_{11}$     & Departure time of $P_1$\\
    $X_1+X_2+Y_{12}$ & Departure time of $P_2$\\
    \hline
    \end{tabular}
    \caption{Notations}
    \label{st2021-50:tab:my_label}
\end{table}
First we present the following result which shall be useful later. For $n>0$,
\begin{align}
    \int_0^{\infty} xe^{-nx}dx = \cfrac{1}{n^2}\label{st2021-50:integrationresult}
\end{align}
The above can be derived using integration by parts as follows
\begin{align}
    \int_0^{\infty} xe^{-nx} dx &= -\cfrac{xe^{-nx}}{n} \biggr \vert_0^{\infty} 
                                   + \cfrac{1}{n} \int_0^{\infty}e^{-nx}dx\\
                                &= -\cfrac{e^{-nx}}{n^2}\biggr \vert_0^{\infty}\\
                                &= \cfrac{1}{n^2}
\end{align}
Next we note that $X_1$, $X_2$ and $X_3$ are identical random variables having Poisson distribution with rate 1. Thus for $i \in \{1,2,3\}$,
\begin{align}
    \lambda &= 1*X_i = X_i\\
    k &= 1\\
    \implies f_{X_i}(x) &= 
    \begin{cases}
        \cfrac{x^1e^{-x}}{1!} = x e^{-x} &x > 0\\
        0                                &otherwise
    \end{cases}
\end{align}
Also $Y_1,...,Y_{12}$ are identical random variables. Thus for $i \in \{1,...,12\}$, as given in question,
\begin{align}
    f_{Y_i}(x) &= 
    \begin{cases}
        e^{-x} & x > 0\\
        0      & otherwise
    \end{cases}\\
    \implies F_{Y_i}(x) &= 
    \begin{cases}
        1-e^{-x} & x > 0\\
        0        & otherwise
    \end{cases}
\end{align}
Now we find $\pr{E_1}$, $\pr{E_2|E_1}$ and $\pr{E_3|E_1E_2}$ in order to find the required probability from eq \eqref{st2021-50:Requiredprobability}.
\begin{align}
    \pr{E_1} &= \pr{Y_1,...,Y_{10} > X_1}\\
             &= \int_{-\infty}^{\infty} \pr{Y_1,...,Y_{10} > x|X_1 = x}\\
             &= \int_{-\infty}^{\infty} (1-F_{Y_1}(x))^{10} f_{X_1}(x)dx\\
             &= \int_0^{\infty} xe^{-11x} dx\\
             &= \cfrac{1}{121}
\end{align}
\begin{multline}
    \pr{E_2|E_1} =\\
    \pr{Y_1,...,Y_{10},X_1+Y_{11} > X_1 + X_2|Y_1,...,Y_{10} > X_1}
\end{multline}
Using memoryless property of exponential random variable,
\begin{align}
    \pr{E_2|E_1} &= \pr{Y_1,...,Y_{11} > X_2}\\
                 &= \int_{-\infty}^{\infty} \pr{Y_1,...Y_{11} > x|X_2 = x}\\
                 &= \int_{-\infty}^{\infty} (1-F_{Y_1}(x))^{11} f_{X_2}(x)dx\\
                 &= \int_{0}^{\infty} x e^{-12x} dx\\
                 &= \cfrac{1}{144}
\end{align}
$\pr{E_3|E_1E_2} = $  
\begin{multline}
    \Pr(min(Y_1,...,Y_{10},X_1+Y_{11},X_1+X_2+Y_{12}) \\
    < X_1+X_2+X_3| Y_1,...,Y_{10},X_1+Y_{11} > X_1+X_2)
\end{multline}
We can simplify and write $\pr{E_3|E_1E_2} = $
\begin{multline}
    1 - \Pr(Y_1,...,Y_{10},X_1+Y_{11},X_1+X_2+Y_{12} \\
    > X_1+X_2+X_3| Y_1,...,Y_{10},X_1+Y_{11} > X_1+X_2)
\end{multline}
Using memoryless property of exponential random variable,
\begin{align}
    \pr{E_3|E_1E_2} &= 1 - \pr{Y_1,...,Y_{12} > X_3}\\
                    &= 1 - \int_{-\infty}^{\infty} \pr{Y_1,...Y_{12} > x|X_3 = x}\\
                    &= 1 - \int_{-\infty}^{\infty} (1-F_{Y_1}(x))^{12} f_{X_3}(x)dx\\
                    &= 1 - \int_{0}^{\infty} x e^{-13x} dx\\
                    &= 1 - \cfrac{1}{169}\\
                    &= \cfrac{168}{169}
\end{align}
Thus on substituting values in \eqref{st2021-50:Requiredprobability}, 
\begin{align}
    \pr{E_1E_2E_3} &= \cfrac{1}{121}\times \cfrac{1}{144}\times \cfrac{168}{169}\\
                   &= 5.7 \times 10^{-5}
\end{align}