
We know that,
\begin{align}
    f_{X_1}(x) = 
    \begin{cases}
    0   & x < 0\\
    \lambda e^{\lambda x} & 0\le x < \infty\\
    \end{cases}
\end{align}
Given, 
\begin{align}
   E(X_1)=\cfrac{1}{\lambda}&=1\\ 
   \implies \lambda &=1
\end{align}
Therefore,
\begin{align}
    f_{X_1}(x) = 
    \begin{cases}
    0   & x < 0\\
    e^{-x} & 0\le x < \infty\\
    \end{cases}
\end{align}
We know that,
\begin{align}
    f_{X_2}(x) = 
    \begin{cases}
    0   & x < 0\\
    \cfrac{x^{\alpha-1}e^{\brak{\frac{-x}{\beta}}}}{\beta^{\alpha}\Gamma(\alpha)} & 0\le x < \infty\\
    \end{cases}
\end{align}
Given, 
\begin{equation}\label{ma2016-47:eq:2.0.4}
    E(X_2)=\alpha \beta =2 
\end{equation}
\begin{equation}\label{ma2016-47:eq:2.0.5}
    V(X_2)=\alpha \beta^{2}=2 
\end{equation}
Solving \ref{ma2016-47:eq:2.0.4} and \ref{ma2016-47:eq:2.0.5}, we get,
$\alpha=2$, $\beta=1$ and $\Gamma(2)=1$\\
Therefore,
\begin{align}
    f_{X_2}(x) = 
    \begin{cases}
    0   & x < 0\\
    xe^{-x} & 0\le x < \infty\\
    \end{cases}
\end{align}
Calculating the CDF of $f_{X_2}(x)$,\\
\begin{align}
    F_{X_2}(x)&= \displaystyle\int\limits_0^x f_{X_2}(x)\\
    F_{X_2}(x)&=
    \begin{cases}
    0 & x<0\\
    \cfrac{\gamma(\alpha,\frac{x}{\beta})}{\Gamma(\alpha)} & 0 \le x <\infty
    \end{cases}
\end{align}
For $\alpha=2$ and $\beta=1$\\
Alternately, we have CDF of $X_1$ and $X_2$ given by 
\begin{align}
    F_{X_1}(x) = 
    \begin{cases}
     0   & x < 0\\
    1-e^{-x} & 0\le x < \infty\\
    \end{cases}
\end{align}
\begin{align}
    F_{X_2}(x) = 
    \begin{cases}
    0   & x < 0\\
    \cfrac{\gamma(2,x)}{\Gamma(2)} & 0\le x < \infty\\
    \end{cases}
\end{align}
Thus, 
\begin{align}
    \pr{X_1\le X_2}&=\displaystyle\int\limits_{-\infty}^{\infty} F_{X_1}(x)f_{X_2}(x)dx\\
                &= \displaystyle\int\limits_0^\infty(1-e^{-x})(xe^{-x})dx\\
                &= \cfrac{3}{4}\\
                &= 0.75
\end{align}