Let $g(X,Y)=X+Y$
We know that,
\begin{align*}
    &E[g(X,Y)]=\int_{-\infty}^{+\infty}\int_{-\infty}^{+\infty}g(x,y)f_{X,Y}(x,y)dxdy\\
\end{align*}
Then,
\begin{align*}
    &E[X+Y]=\int_{-\infty}^{+\infty}\int_{-\infty}^{+\infty}(x+y)f_{X,Y}(x,y)\,dxdy\\
    &=\int_{0}^{+\infty}\int_{0}^{+\infty}(x+y)f_{X,Y}(x,y)\,dxdy\\
    &=\int_{0}^{+\infty}\left(\int_{0}^{+\infty}xf_{X,Y}(x,y)\,dx+\int_{0}^{+\infty}yf_{X,Y}(x,y)\,dx\right)\,dy
\end{align*}
First we will calculate the $\int_{0}^{+\infty}yf_{X,Y}(x,y)\,dx$,  $\int_{0}^{+\infty}xf_{X,Y}(x,y)\,dx$ seperately.\\
consider,
\begin{align*}
    &\int_{0}^{+\infty}yf_{X,Y}(x,y)\,dx\\
    &=\int_{0}^{y}ye^{-y}(1-e^{-x})\,dx+\int_{y}^{+\infty}ye^{-x}(1-e^{-y})\,dx\\
    &=(ye^{-y})(y+e^{-y}-1)+y(1-e^{-y})e^{-y}\\
    &=y^2e^{-y}
\end{align*}
So,
\begin{align}
    \tag{37.1}
    \int_{0}^{+\infty}yf_{X,Y}(x,y)\,dx=y^2e^{-y}
\end{align}
Now consider,
\begin{align*}
  &\int_{0}^{+\infty}xf_{X,Y}(x,y)\,dx\\
  &=\int_{0}^{y}xe^{-y}(1-e^{-x})\,dx+\int_{y}^{+\infty}xe^{-x}(1-e^{-y})\\
  &=e^{-y}\left(\frac{y^2}{2}+e^{-y}(y+1)-1\right)+(1-e^{-y})(e^{-y}(y+1))\\
  &=\frac{y^2e^{-y}}{2}+ye^{-y}
\end{align*}
So,
\begin{align}
    \tag{37.2}
    \int_{0}^{+\infty}xf_{X,Y}(x,y)\,dx=\frac{y^2e^{-y}}{2}+ye^{-y}
\end{align}
From Eq 37.1 and 37.2
\begin{align*}
    &E[X+Y]=\int_{0}^{+\infty}\left(\frac{y^2e^{-y}}{2}+ye^{-y}+y^2e^{-y}\right)\,dy\\
    &=\int_{0}^{+\infty}\left(\frac{3}{2}y^2e^{-y}+ye^{-y}\right)\,dy\\
    &=\left(-\frac{3}{2}(y^2+2y+2)e^{-y}+(-e^{-y}(y+1))\right)\Biggr|_{0}^{+\infty}\\
    &=\frac{3}{2}\times2+1\\
    &=4
\end{align*}
So,
\begin{align*}
  &E[X+Y]=4
\end{align*}