%
Given,
\begin{align}
   \label{ma2010-1:(2.0.1)} \pr{E} &= 0.4 \\
   \label{ma2010-1:(2.0.2)} \pr{E+F} &= 0.8 \\
    \pr{E|F} &= 0.3
\end{align}
By definition,
\begin{align}
    \pr{E|F} &= \frac{\pr{EF}}{\pr{F}} \\
    \implies \pr{EF} &= \pr{E|F} \times \pr{F} \\
    \label{ma2010-1:(2.0.6)}\implies \pr{EF} &= 0.3 \times \pr{F}
\end{align}
Now using the identity,
\begin{align}
    \pr{E+F} &= \pr{E} + \pr{F} - \pr{EF}
\end{align}
From \eqref{ma2010-1:(2.0.1)},\eqref{ma2010-1:(2.0.2)} and \eqref{ma2010-1:(2.0.6)}
\begin{align}
    \implies 0.8 &= 0.4 + \pr{F} - \brak{0.3 \times \pr{F}} \\
    \implies 0.4 &= \brak{1-0.3} \times \pr{F} \\
    \implies \pr{F} &= \frac{0.4}{0.7}
\end{align}
\begin{equation}
    \boxed{\pr{F} = \frac{4}{7}}
\end{equation}