Given
\begin{enumerate}
\item $\pr{E}=0.4$
\item $\pr{F}=0.3$
\item $\pr{F|E}=3 \pr{F|E'}$
\end{enumerate}
From given data
\begin{align}
\pr{F|E}=3 \pr{F|E'}\\
\frac{\pr{FE}}{\pr{E}}=3\times \frac{\pr{FE'}}{\pr{E'}}\\
\pr{EF}=2\times\pr{E'F}\label{eq:fac}
\end{align}
We know that
\begin{align}
\pr{F}=\pr{EF}+\pr{E'F} \label{eq:refer}
\end{align}
Using \eqref{eq:fac} and \eqref{eq:refer}, we get
\begin{align}
\pr{F}=\frac{3}{2}\times\pr{EF}\\
\frac{\pr{EF}}{\pr{F}}=\frac{2}{3}\\
\pr{E|F}=\frac{2}{3}\approx 0.66
\end{align}