The expectation operator, 
\begin{align}
    E\brak{X_1 + .... + X_n}
    &= E\brak{X_1} +.....+ E\brak{X_n} \label{ma2016-46:eq 2.0.1}
\end{align}
We know that, 
\begin{align}
    E\brak{X} 
    &= \sum_{i = 1}^\infty x_i\Pr\brak{X = x_i}\\
    &=  \sum_{i = 1}^\infty k_i\Pr\brak{X = k_i} \label{ma2016-46:eq 2.0.3}
\end{align}
So now, 
\begin{align}
    E\brak{X_1} = k_1\Pr\brak{X = k_1} = 1 \brak{\frac{1}{2}} \label{ma2016-46:eq 2.0.4}
\end{align}
Similarly, 
\begin{align}
    E\brak{X_2} = k_2\Pr\brak{X = k_2} = 2 \brak{\frac{1}{2}}^{2} \label{ma2016-46:eq 2.0.5}
\end{align}
and the pattern follows.
Let 
\begin{align}
    E\brak{X_1 + .... + X_n} = S \label{ma2016-46:eq 2.0.6}
\end{align}
By substituting \eqref{ma2016-46:eq 2.0.4} and \eqref{ma2016-46:eq 2.0.5} in \eqref{ma2016-46:eq 2.0.1}
\begin{align}
    S = 1 \brak{\frac{1}{2}} + 2 \brak{\frac{1}{2}}^{2} + 3\brak{\frac{1}{2}}^{3} + ..... \label{ma2016-46:eq 2.0.7}
\end{align}
Dividing by 2 on both sides 
\begin{align}
   \frac{S}{2} =  0\brak{\frac{1}{2}} + 1\brak{\frac{1}{2}}^{1} + 2\brak{\frac{1}{2}}^{2} + ..... \label{ma2016-46:eq 2.0.8}
\end{align}
Subtracting \eqref{ma2016-46:eq 2.0.8} from \eqref{ma2016-46:eq 2.0.7}
\begin{align}
    \frac{S}{2} 
    &= \frac{1}{2} + \frac{1}{2}^{2} + \frac{1}{2}^{3}  + ....\\
    &= \frac{1/2}{1-1/2} \\
    &= 1
\end{align}
Therefore, from \eqref{ma2016-46:eq 2.0.6}
\begin{align}
    E \brak{X_1 + X_2 +..... + X_n} = 2
\end{align}
