
If E and F are independent, E' and F' are also independent.\\So,
\begin{align}
    \pr{EF}&=\pr{E}\pr{F}\nonumber\\
            &=\frac{1}{6}\label{ma1999-28:a}\\
    \pr{E'F'}&=\pr{E'}\pr{F'}\nonumber\\
            &=\brak{1-\pr{E}}\brak{1-\pr{F}}\nonumber\\
            &=\frac{1}{3}\label{ma1999-28:c}
\end{align}
From $\eqref{ma1999-28:a}$ and $\eqref{ma1999-28:c}$
\begin{align}
    \pr{E}+\pr{F}&=\frac{5}{6}\label{ma1999-28:b}
\end{align}
From $\eqref{ma1999-28:a}$ and $\eqref{ma1999-28:b}$,
\begin{align}
    \pr{E}\brak{\frac{5}{6}-\pr{E}}&=\frac{1}{6}\nonumber\\
\equiv \pr{E}&=\frac{1}{3}\text{or}\frac{1}{2}\nonumber
\end{align}
$\pr{E}=\frac{1}{2}$ satisfies $\pr{E}>\pr{F}$ while $\pr{E}=\frac{1}{3}$ does not.\\
$\therefore \pr{E}=\frac{1}{2}$\\
\solution{Option A}