
Given A and B are two events,\\
We know that,
\begin{align}
    A&=A(B+\bar{B})\\
    &=AB+A\bar{B}
\end{align}
Since $AB$ and $A\bar{B}$ are disjoint events,
\begin{align}
    \Pr{(A)}=\Pr{(AB)}+\Pr{(A\bar{B})}
\end{align}
Hence,
\begin{equation}
    \Pr(A\bar{B})=\Pr{(A)}-\Pr{(AB)}\label{ma1997-18:eq:2.0.4}
\end{equation}
Since $B$ and $\bar{B}$ are disjoint events,
\begin{align}
    \Pr{(B)}+\Pr{(\bar{B})}=1\\
    \Pr{(\bar{B})}=1-\Pr{(B)}\label{ma1997-18:eq:2.0.6}
\end{align}
We know that,
\begin{equation}
\Pr{(A|\bar{B})}=\frac{\Pr{(A\bar{B})}}{\Pr{(\bar{B})}} \label{ma1997-18:eq:2.0.7}    
\end{equation}
From \eqref{ma1997-18:eq:2.0.6} and \eqref{ma1997-18:eq:2.0.4}
\begin{align}
    \frac{\Pr(A)-\Pr(AB)}{1-\Pr{(B)}}=\frac{\Pr{(A\bar{B})}}{\Pr{(\bar{B})}}
\end{align}
From \eqref{ma1997-18:eq:2.0.7}
\begin{equation}
    \frac{\Pr(A)-\Pr(AB)}{1-\Pr{(B)}}=\Pr{(A|\bar{B})}
\end{equation}
Hence \textbf{option A is correct}